
\input{header}

\begin{document}


\title{Lecture 5}

\date{Mar 25, 2024}

\maketitle


	Last time we constructed a homomorphism $\phi: Z(\mfg) \to \Sym(\mft)$ fitting into the following diagram
	\begin{equation}
		\label{eqn-phi}
		\xymatrix{
			Z(\mfg) 
				\ar[r]^-\phi
				\ar[rd]_-{\chi_\lambda=\xi_{-,\lambda}}
			& \Sym(\mft) \ar[d]^-{\ev_\lambda} \\
			& k_\lambda,
		}
	\end{equation}
	where for any $\lambda\in \mft^*$, $\chi_\lambda=\xi_{-,\lambda}$ is the central character of the Verma module $M_\lambda$. We stated the following result, which will be proved today.

	\begin{thm}[Harish-Chandra]
	\label{thm-HC}
		The homomorphism $\phi$ induces an isomorphism
		\[
			\phi_\HC: Z(\mfg)  \xrightarrow{\sim} \Sym(\mft)^{W_\bullet}
		\]
		from $Z(\mfg)$ to the invariance of $\Sym(\mft)$ with respect to the dotted $W$-action.

	\end{thm}

\section{Step 1: image is \texorpdfstring{$W_\bullet$}{W.}-invariant}

	Let us first prove the image of $\phi$ is indeed contained in $\Sym(\mft)^{W_\bullet}$. Since $W$ is generated by simple reflections $s_\alpha$, $\alpha\in \Delta$, we only need to show $\phi(z) = s_\alpha \cdot \phi(z)$ for any $z\in Z(\mfg)$. In other words, we need to show
	\begin{equation}
		\label{eqn-1}
		\ev_\lambda(\phi(z)) = \ev_\lambda(s_\alpha \cdot \phi(z))
	\end{equation}
	for any $\lambda\in \mft^*$. In fact, we only need to prove this for a Zariski dense subset of $\mft^*$. Let us first give this dense subset. The following result is obvious after drawing a picture.

	\begin{lem}
		Let $\alpha\in \Delta$ be a simple root. The subset $\{ \lambda\in \mft^*\,\vert\, \langle \lambda+\rho, \check\alpha \rangle \in \mBZ^{\ge 0} \}$\footnote{In other words, $\lambda+\rho$ is \textbf{dominant and integral}.} is a Zariski dense subset of $\mft^*$.
	\end{lem}

	\begin{exam}
		For $\mfg=\sl_2$, this subset is $\mBZ^{\ge -1}\subset \mBA^1$. In fact, in [Exam. 15, Lect. 4], we have used this subset to show the image of $\phi:Z(\sl_2) \to k[h]$ is invariant under $h\mapsto -h-2$. The argument below is an immediate generalization.
	\end{exam}

	\begin{lem}
		\label{lem-Verma-simple-reflection}
		Let $\alpha\in \Delta$ be a simple root and $\lambda\in \mft^*$. Suppose $\langle \lambda+\rho, \check\alpha \rangle \in \mBZ^{\ge 0} $. Then $M_\lambda$ contains $M_{s_\alpha\cdot \lambda}$ as a submodule.
	\end{lem}

	\begin{cor}
		The image of $\phi: Z(\mfg)\to \Sym(\mft)$ is indeed contained in $\Sym(\mft)^{W_\bullet}$. 
	\end{cor}

	\proof
		By previous discussion, we only need to prove \eqref{eqn-1} for $\alpha$ and $\lambda$ satisfying the assumption of Lemma \ref{lem-Verma-simple-reflection}. By \eqref{eqn-phi}, the LHS and RHS of \eqref{eqn-1} are exactly the central character of $M_\lambda$ and $M_{s_\alpha\cdot \lambda}$. Now Lemma \ref{lem-Verma-simple-reflection} implies they are equal because the central character of a module is equal to the central character of any nonzero submodule of it.

	\qed

	\proof[Proof of Lemma \ref{lem-Verma-simple-reflection}]
		Recall 
		\[
			s_\alpha(\lambda) = \lambda - 2\frac{(\lambda,\alpha)}{(\alpha,\alpha)}\alpha = \lambda - \langle \lambda,\check\alpha  \rangle \alpha.
		\]
		It follows that
		\[
			s_\alpha \cdot \lambda = \lambda - \langle \lambda+\rho, \check\alpha \rangle  \alpha  = \lambda - m\alpha
		\]
		for $m\in \mBZ^{\ge 0}$. The lemma is obvious for $m=0$. We assume $m>0$. Then we have $\langle \lambda,\check \alpha \rangle = m-1$ because $\langle \rho,\check\alpha \rangle = 1$ (see \cite[Cor. to Lem. 10.2(B)]{H1}).

		Let $f_\alpha\in \mfn^-$ be a nonzero vector of weight $-\alpha$. Consider the vector $f_\alpha^m \cdot v_\lambda$, which is of weight $\lambda-m\alpha=s_\alpha \cdot \lambda$. We only need to show
		\[
			\mfn \cdot (f_\alpha^m \cdot v_\lambda) =0.
		\]
		Indeed, if this is true, the map $k_{s_\alpha \cdot \lambda}\to M_\lambda,\; c\mapsto c(f_\alpha^m \cdot v_\lambda)$ is $\mfb$-linear, and thereby induces a $\mfg$-linear map $M_{s_\alpha\cdot \lambda}\to M_{\lambda}$. This map is injective because as a morphism between $U(\mfn^-)$-modules, it is given by $ -\cdot f_\alpha^m : U(\mfn^-) \to U(\mfn^-)$, which is injective by the PBW theorem.

		It remains to show $\mfn$ annihilates $f_\alpha^m \cdot v_\lambda$. For each simple root $\beta\in \Delta$, let $e_\beta\in \mfn$ be a nonzero vector of weight $\beta$. Note that the vectors $(e_\beta)_{\beta\in \Delta}$ generate $\mfn$ under Lie brackets\footnote{Because $[\mfg_\alpha,\mfg_\beta] = \mfg_{[\alpha,\beta]}$ whenever $\alpha,\beta,\alpha+\beta\in \Phi^+$.}. Hence we only need to show $e_\beta\cdot f_\alpha^m \cdot v_\lambda =0$. There are two cases:
		\begin{itemize}
			\item 
				If $\alpha\neq \beta$, then $[e_\beta,f_\alpha]=0$\footnote{Otherwise it is a nonzero vector with weight $\beta-\alpha$ but the latter is not a root because $\Phi = \Phi^+ \sqcup \Phi^-$.} and
				\[
					e_\beta\cdot f_\alpha^m \cdot v_\lambda = f_\alpha^m \cdot e_\beta \cdot v_\lambda = 0
				\]
				because $\mfn \cdot v_\lambda =0$.
			\item
				If $\alpha = \beta$, $[e_\alpha,f_\alpha]\in \mft$ is propotionate to $\check \alpha$ (see \cite[Prop. 8.3(d)]{H1}). Rescale $e_\alpha$, we may assume $[e_\alpha,f_\alpha ]= \check \alpha$. Then $[\check \alpha ,f_\alpha ]= \langle -\alpha,\check\alpha\rangle f_\alpha = -2f_\alpha$. Now the following calculation is essentially that in [Exe. 24, Lect. 2]. We have
				\[
					e_\alpha\cdot f_\alpha^m \cdot v_\lambda  = \sum_{1\le i\le m} f_\alpha^{m-i}\cdot [e_\alpha,f_\alpha] \cdot f_\alpha^{i-1}\cdot v_\lambda + f_\alpha^m \cdot e_\alpha \cdot v_\lambda.
				\]
				Recall we have $e_\alpha \cdot v_\lambda=0$. Also,
				\[
					\check \alpha \cdot f_\alpha^j = \sum_{1\le i\le j} f_\alpha^{j-i}\cdot [\check \alpha, f_\alpha] \cdot f_\alpha^{i-1} + f_\alpha^j  \cdot \check \alpha  = -2j f_\alpha^j +  f_\alpha^j  \cdot \check \alpha.
				\]
				Hence
				\[
					e_\alpha\cdot f_\alpha^m \cdot v_\lambda  = \sum_{1\le i\le m} (-2(i-1)f_\alpha^{m-1}+ f_\alpha^{m-1}\cdot \check\alpha ) v_\lambda = \big(-m(m-1) + m\langle \lambda,\check\alpha\rangle \big)v_\lambda = 0
				\]
				as desired.
		\end{itemize}
		
	\qed[Lemma \ref{lem-Verma-simple-reflection}]

\section{Step 2: Filtrations}
	
	By Step 1, we have a homomorphism
	\[
		\phi_\HC: Z(\mfg) \to \Sym(\mft)^{W_\bullet}.
	\]
	In this step, we equip both sides with filtrations, and show $\phi_\HC$ is compatible with them. The punchline is the following easy fact:

	\begin{facts}
		Let $V_1$ and $V_2$ be two vector spaces equipped with $\mBZ^{\ge 0}$-indexed (exhausted) filtrations. Suppose $\varphi:V_1\to V_2$ is a $k$-linear map compatible with the filtrations. Then $\varphi$ is an isomorphism iff $\gr^\bullet \varphi: \gr^\bullet V_1 \to \gr^\bullet V_2$ is so.
	\end{facts}

	\begin{constr}
		The PBW filtration on $U(\mfg)$ induces a filtration on $Z(\mfg)$ with $\mbF^{\le i} Z(\mfg):= Z(\mfg)\cap \mbF^{\le i}U(\mfg)$. Note that $\gr^\bullet Z(\mfg)$ is a subalgebra of $\gr^\bullet U(\mfg) \simeq \Sym(\mfg)$.
	\end{constr}

	\begin{constr}
		The PBW filtration on $U(\mft)\simeq \Sym(\mft)$ is preserved by the dotted $W$-action. Hence it induces a filtration on $U(\mft)^{W_\bullet}$\footnote{Note that $\gr^\bullet U(\mft)$ is also isomorphic to $\Sym(\mft)$. To distinguish them, we always use $U(\mft)$ to denote the filtered commutative ring while use $\Sym(\mft)$ to denote the graded commutative ring.}.
	\end{constr}

	\begin{warn}
		The \emph{dotted} $W$-action on $\Sym(\mft)$ does not preserve the grading. But the usual (linear) $W$-action does.
	\end{warn}

	\begin{lem}
		The homomorphism $\phi_\HC: Z(\mfg) \to U(\mft)^{W_\bullet}$ is compatible with the above filtrations.
	\end{lem}

	\proof
		This is obvious from the description of $\phi$ as
		\[
			Z(\mfg) \inj U(\mfg) \surj k\ot_{U(\mfn^-)} U(\mfg) \ot_{U(\mfn)} k \simeq U(\mft).
		\]
	\qed

\section{Step 3: Calculating the graded pieces}
	
	\begin{constr}
	\label{constr-adj-action-sym}
		Recall $\Sym(\mfg)$ has a natural $\mfg$-module structure constructed as follows. For any $V\in \mfg$, there is a natural $\mfg$-module structure on $V^{\otimes n}$ given by 
		\[
			\mfg \mt V^{\otimes n} \to V^{\otimes n},\; (x, \ot_i v_i)\mapsto \sum_i ( v_1\ot \cdots\ot v_{i-1}\ot (x\cdot v_i) \ot v_{i+1}\cdots \ot v_n ).
		\]
		This action is compatible with the symmetric group $\Sigma_n$-action on $V^{\otimes n}$ and thereby induces a $\mfg$-module structure on $\Sym^n(V)$. Taking direct sum, we obtain a $\mfg$-module structure on $\Sym(V)$. 

		In the case $V=\mfg$, to distinguish with the multiplication structure on $\Sym(\mfg)$, we denote this action by
		\[
			\mfg \times \Sym(\mfg) \to \Sym(\mfg) ,\; (x,u)\mapsto \ad_x(u),
		\]
		and call it the \textbf{adjoint action}.

		Note that by definition, for $x\in \mfg$ and $u,v\in \Sym(\mfg)$, we have
		\[
			\ad_x(u\cdot v) = \ad_x(u)\cdot v + u\cdot \ad_x(v).
		\]
		In particular, the \emph{$\mfg$-invariance} 
		\[
			\Sym(\mfg)^\mfg:= \{ u\in \Sym(\mfg)\,\vert\, \ad_x(u)=0\textrm{ for any }x\in \mfg \}
		\]
		is a subalgebra of $\Sym(\mfg)$.
	\end{constr}

	\begin{lem}
	\label{lem-Zg-fil}
		There is a unique dotted graded isomorphism making the following diagram commute
		\[
			\xymatrix{
				\gr^\bullet Z(\mfg) \ar@{.>}[r]^-\simeq \ar[d]^-\subset
				& \Sym(\mfg)^\mfg \ar[d]^-\subset \\
				\gr^\bullet U(\mfg) \ar[r]^-\simeq 
				& \Sym(\mfg),
			}
		\]
		where the bottom isomorphism is given by the PBW theorem.
	\end{lem}

	To prove this lemma, we use the following exercise:

	\begin{exe}
		This is \red{Homework 2, Problem 4}. Prove: the adjoint $\mfg$-action on $U(\mfg)$, i.e.,
		\[
			\mfg \times U(\mfg) \to U(\mfg),\; (x,u)\mapsto \ad_x(u)=[x,u],
		\]
		preserves each $\mbF^{\le n}U(\mfg)$, and the induced $\mfg$-action on $\gr^\bullet(U(\mfg)) \simeq \Sym(\mfg)$ is the adjoint action in Construction \ref{constr-adj-action-sym}.
	\end{exe}


	\proof[Proof of Lemma \ref{lem-Zg-fil}]
		By the above exercise, we have a short exact sequence of \emph{finite-dimensional} $\mfg$-modules:
		\[
			0 \to \mbF^{\le n-1} U(\mfg) \to \mbF^{\le n} U(\mfg)  \to \Sym^n(\mfg) \to 0.
		\]
		Since $\mfg\hmod_\mathsf{fd}$ is semisimple, this short exact sequence splits. Hence taking $\mfg$-invariance, we obtain\footnote{
			Warning: in general, taking invariance is only \emph{left exact}. (Memory method: it is given by $\Hom_{\mfg}(k,-)$.) Hence we need the existence of a splitting.
		}
		\[
			0 \to \mbF^{\le n-1} Z(\mfg) \to \mbF^{\le n} Z(\mfg) \to \Sym^n(\mfg)^\mfg \to 0
		\]
		This gives the desired isomorphism $\gr^n Z(\mfg) \simeq \Sym^n(\mfg)^\mfg$.

	\qed[Lemma \ref{lem-Zg-fil}]
	
	A similar proof\footnote{Note that $\Rep(W)_\mathsf{fd}$ is also semisimple} gives:

	\begin{lem}
	\label{lem-UtW-fil}
		There is a unique dotted graded isomorphism making the following diagram commute
		\[
			\xymatrix{
				\gr^\bullet (U(\mft)^{W_\bullet}) \ar@{.>}[r]^-\simeq \ar[d]^-\subset
				& \Sym(\mft)^W \ar[d]^-\subset \\
				\gr^\bullet U(\mft) \ar[r]^-\simeq 
				& \Sym(\mft),
			}
		\]
		where the right-top corner is the invariance for the \emph{linear} $W$-action on $\Sym(\mft)$.
	\end{lem}

	Combining the above two lemmas, we obtain:

	\begin{cor}
		There is a unique dotted graded homomorphism making the following diagram commute
		\[
			\xymatrix{
				\gr^\bullet Z(\mfg) \ar[r]^-\simeq \ar[d]^-{\gr^\bullet \phi_\HC}
				& \Sym(\mfg)^\mfg \ar@{.>}[d]^-{\phi_\cl} \\
				\gr^\bullet (U(\mft)^{W_\bullet})  \ar[r]^-\simeq 
				& \Sym(\mft)^W.
			}
		\]
	\end{cor}

\section{Step 4: Chevalley isomorphism}
	It remains to show
	\[
		\phi_\cl: \Sym(\mfg)^\mfg \to \Sym(\mft)^W
	\]
	is an isomorphism. Let us first give an explicit construction of this homomorphism. We need the following characterization of $\phi$.

	\begin{constr}
		Consider the composition
		\[
			Z(\mfg) \inj U(\mfg) \surj  U(\mfg) \ot_{U(\mfn)} k.
		\]
		With respect to the adjoint $\mft$-action, the source has weight $0$. Hence the composition factors through the $0$-weight subspace of the target, which is exactly $U(\mfb) \ot_{U(\mfn)} k \simeq U(\mft)$. By definition, the obtained map
		\[
			Z(\mfg) \to U(\mft)
		\] 
		is just $\phi$.
	\end{constr}

	\begin{constr}
		It follows $\phi_\cl$ can be constructed as follows. Consider the composition
		\begin{equation}
			\label{eqn-3}
			\Sym(\mfg)^\mfg \inj \Sym(\mfg) \surj \Sym(\mfg/\mfn).
		\end{equation}
		It factors through $\Sym(\mfb/\mfn)\simeq \Sym(\mft)$. The obtained map
		\[
			\Sym(\mfg)^\mfg  \to  \Sym(\mft)
		\]
		can be identified with $\gr^\bullet \phi$. Since $\phi$ factors through $U(\mft)^{W_\bullet}$, the map $\gr^\bullet \phi$ factors through $\gr^\bullet(U(\mft)^{W_\bullet}) \simeq \Sym(\mft)^W$. The obtained map 
		\[
			\Sym(\mfg)^\mfg  \to  \Sym(\mft)^W
		\]
		is just $\phi_\cl$.
	\end{constr}
 
	\begin{rem}
		\label{rem-geometric-Chevalley}
		The geometric meaning of the above construction is as follows. 

		Note that $\Sym(\mfg)^\mfg = \Sym(\mfg)^G$ because $G$-invariance is equal to $\mfg$-invariance\footnote{Because $\Rep(G) \to \mfg\hmod$ is fully faithful when $G$ is connected.}. Hence \eqref{eqn-3} corresponds to the morphisms
		\[
			(\mfg/\mfn)^* \to \mfg^* \to \mfg^*/\!/G.
		\]
		Since $\gr^\bullet \phi$ factors through $\gr^\bullet(U(\mft)^{W_\bullet}) \simeq \Sym(\mft)^W$. The above composition factors through $(\mfg/\mfn)^* \to (\mfb/\mfn)^* \simeq \mft^* \to \mft^*/\!/W$. In other words, we have
		\[
			\xymatrix{
				(\mfg/\mfn)^* \ar[r] \ar[d] & \mfg^*/\!/G  \\
				\mft^* \ar[r] & \mft^*/\!/W \ar@{.>}[u]
			}
		\]
		such that the dotted arrow is given by $\Spec(\phi_\cl)$.

		It is convenient to get rid of the dual spaces using the Killing form. Namely, $\Kil$ induces an isomorphism $\mfg\simeq \mfg^*$ compatible with the $G$-actions, while $\Kil|_\mft$ induces an isomorphism $\mft\simeq \mft^*$ compatible with the $W$-actions\footnote{Both claims follow from the fact that $\Kil$ is invariant with respect to the adjoint $\mfg$-action and thereby to the adjoint $G$-action. Here we use $W\simeq N_G(T)/T$.}. Via the first isomorphism, the subspaces $\mfn\subset \mfb\subset \mfg$ corresponds to $(\mfg/\mfb)^*\subset (\mfg/\mfn)^* \subset \mfg$. Then the above commutative diagram is identified with
		\begin{equation}
			\label{eqn-square}
			\xymatrix{
				\mfb \ar[r] \ar[d] & \mfg/\!/G  \\
				\mft \ar[r] & \mft/\!/W. \ar@{.>}[u]
			}
		\end{equation}
		We abuse notations and also view the dotted arrow as $\Spec(\phi_\cl)$.

	\end{rem}

	\begin{rem}
		Since the projection $\mfb\to \mft$ has a splitting $\mft \to \mfb$. The above claim implies $\mft \to \mfg \to \mfg/\!/G$ factors through $\mft/\!/ W$. We can also prove this using group-theoretic method. Namely, consider the normalizer $N_G(T)$ of $T$ insider $G$. Recall we have $W\simeq N_G(T)/T$ such that the linear $W$-action on $\mft$ can be identified with the adjoint action of $N_G(T)/T$. Then the morphism $\mft \to  \mfg/\!/G$ factors through $\mft/\!/ W$ because $N_G(T)$ is a subgroup of $G$.
	\end{rem}

	\begin{warn}
		I do not know any group-theoretic proof of \eqref{eqn-square}. This is because not $\mfb \to \mfg/G$ (the quotient stack) does not factor through $\mft$: two elements in $\mfb$ that have the same image in $\mft$ are not necessarily conjugate to each other.
	\end{warn}

	\begin{thm}[Chevalley]
		The homomorphism 
		\[
			\phi_\cl: \Sym(\mfg)^\mfg  \to  \Sym(\mft)^W
		\]
		is an isomorphism. In other words, the natural morphism $\mft/\!/ W \to \mfg/\!/G$ is an isomorphism.
	\end{thm}

	\proof
		As in Remark \ref{rem-geometric-Chevalley}, we can identify $\phi_\cl$ with the restriction map $\Fun(\mfg)^G \to \Fun(\mft)^W$, which is also $\Sym(\mfg^*)^G \to \Sym(\mft^*)^W$.

		This map is injective because if an adjoint-invariant function on $\mfg$ vanishes on $\mft$, then it vanishes on each semisimple elements. But the latter are Zariski dense in $\mfg$.

		To prove the surjectivity, we first find generators of $\Sym(\mft^*)^W$ as follows. Recall the subset $P^+$ of \textbf{dominant integral weights}, i.e.,
		\[
			P^+ := \{ \lambda\in \mft^*\,\vert\, \langle\lambda,\check\alpha\rangle \in \mBZ^{\ge 0} \textrm{ for all }  \alpha\in \Delta \}.
		\]
		Note that $P^+$ spans $\mft^*$. In fact, for each $\alpha\in \Delta$, we can find \textbf{fundamental dominant weights} $\omega_\alpha$ such that
		\[
			\langle \omega_\alpha,\check \beta \rangle = \delta_{\alpha\beta},\; \alpha,\beta\in \Delta.
		\]
		Then $\{\omega_\alpha\}$ is a basis of $\mft^*$ and $P^+= \mBZ^{\ge 0}\{\omega_\alpha\}$. A direct calculation shows that $\{\lambda^n\,\vert\, \lambda\in P^+ \}$ span $\Sym^n(\mft^*)$. Hence the sums
		\[
			b_{\lambda,n}:= \sum_{w\in W} w( \lambda^n ),\; \lambda \in P^+, n\ge 0
		\]
		span $\Sym(\mft^*)^W$.
		
		It remains to show each $b_{\lambda,n}$ is contained in the image of $\phi_\cl$. We need the following well-known fact.

		\begin{thm}[Weyl]
			For any $\lambda\in P^+$, there is a unique finite-dimensional irreducible $\mfg$-module $L_\lambda$ with higheset weight $\lambda$.
		\end{thm}

		For $\lambda \in P^+, n\ge 0$, consider the function $a_{\lambda,n}\in \Fun(\mfg) $ defined by
		\[
			a_{\lambda,n}(x):=\tr(x^n; L_\lambda),
		\]
		i.e., its value at any $x\in \mfg$ is the trace of the action of $x^n$ on $L_\lambda$. It is easy to see $a_{\lambda,n}$ is $\mfg$-invariant\footnote{Recall $L_\lambda$ is $G_\mathsf{sc}$-integrable ([Thm. 47, Lect. 3]). Hence $a_{\lambda,n}$ is $G_\mathsf{sc}$-invariant, and thereby $\mfg$-invariant.
		} and thereby $G$-invariant. 

		Now the following exercise implies each $b_{\lambda,n}$ is contained in the image of $\phi_\cl$. Indeed, this follows from induction on $\lambda$ with respect to the partial ordering $\prec$\footnote{Recall $\lambda'\preceq\lambda$ iff $\lambda-\lambda' \in \mBZ^{\ge 0}\Phi^+$. See [Defn. 22, Lect. 2].}.

		\begin{exe}
			This is \red{Homework 2, Problem 5}. Let $\lambda \in P^+$ be a dominant integral weight and $n\ge 0$. Prove there exists scalars $c_{\lambda'} \in k$, $\lambda' \prec \lambda$ such that
			\[
				\phi_\cl(a_{\lambda,n}) = a_{\lambda,n}|_{\mft} = \frac{1}{\#\mathsf{Stab}_W(\lambda)}b_{\lambda,n} + \sum_{\lambda' \prec \lambda} c_{\lambda'}b_{\lambda',n},
			\]
			where $\mathsf{Stab}_W(\lambda)\subset W$ is the stablizer of the $W$-action at $\lambda$.

		\end{exe}

	\qed

	Combining all the previous discussion, we finish the proof of Theorem \ref{thm-HC}.

\section{More on the quotient \texorpdfstring{$\mft/\!/W$}{t//W}}

	We state some results on $\mft/\!/W\simeq \mft/\!/W_\bullet$ without proof.

	\begin{prop}[{\!\!\cite[Sect. 1.10]{H2}}]
		The morphism $\varpi:\mft \to \mft/\!/W_\bullet$ is surjective, and $W_\bullet$ acts transitively on the fiber at each closed point.
	\end{prop}

	\begin{rem}
		In other words, any character $\chi:Z(\mfg) \to k$ is the central character $\chi_\lambda$ for some Verma module $V_\lambda$, and $\chi_\lambda =\chi_\mu$ iff $\mu=w\cdot \lambda$ for some $w\in W$.
	\end{rem}

	\begin{cor}[Linkage principle]
	Verma modules $M_\lambda$ and $M_\mu$ belong to the same block iff $\mu = w\cdot \lambda$ for some $w\in W$. In particular, there are only finitely many Verma modules and irreducible objects\footnote{Recall $M_\lambda$ has a unique irreducible quotient $L_\lambda$, and all irreducible objects of $\mCO$ are of this form. See [Thm. 25, Prop. 31, Lec. 2].} in each block.
	\end{cor}

	\begin{prop}[{\!\!\cite[Sect. 7]{G}}]
		We have
		\begin{itemize}
			\item[(1)]
				The schemes $ \mft/\!/W \simeq \mfg/\!/G$ are smooth.
			\item[(2)]
				The map $\mft \to  \mft/\!/W$ is flat.
			\item[(3)]
				The map $\mfg \to  \mfg/\!/G$ is flat.
		\end{itemize}
	\end{prop}


	
\begin{thebibliography}{Yau}

	\bibitem[G]{G} Gaitsgory, Dennis. Course Notes for Geometric Representation Theory, 2005, available at \url{https://people.mpim-bonn.mpg.de/gaitsgde/267y/catO.pdf}.

	\bibitem[H1]{H1} Humphreys, James E. Introduction to Lie algebras and representation theory. Vol. 9. Springer Science \& Business Media, 2012.

	\bibitem[H2]{H2} Humphreys, James E. Representations of Semisimple Lie Algebras in the BGG Category $\mathcal{O} $. Vol. 94. American Mathematical Soc., 2008.

\end{thebibliography}

\end{document} 


